src/simple-proof/proof/OperationalSemantics.v
@@ -4,48 +4,64 @@ Require Import Coq.Program.Equality.
 Require Import LibLN.
 Require Import Definitions Binding.
 
-(** * Stack-Based Operational Semantics *)
+Fixpoint defs_update (ds: defs) (a: trm_label) (t: trm) : defs :=
+  match ds with
+  | defs_nil => defs_nil
+  | defs_cons ds' (def_typ A T)  =>
+    defs_cons (defs_update ds' a t) (def_typ A T)
+  | defs_cons ds' (def_trm a' t')  =>
+    If a = a' then defs_cons ds' (def_trm a t') else defs_cons (defs_update ds' a t) (def_trm a' t')
+end.
 
-Reserved Notation "t1 '|->' t2" (at level 40, t2 at level 39).
+Reserved Notation "t1 '|->l' t2" (at level 40, t2 at level 39).
 
-Inductive red : sta * trm -> sta * trm -> Prop :=
+Definition call_stack := (list (var * trm_label)).
+
+Inductive red_l : sta * trm * (list (var * trm_label)) -> sta * trm * (list (var * trm_label)) -> Prop :=
 (** [s(x) = nu(T)...{a = t}...]  #<br>#
     [―――――――――――――――――――――――――]  #<br>#
-    [(s, x.a) |-> (s, t)      ]  *)
-| red_sel : forall x m s t T ds,
+    [(s, x.a) |->l (s, t)      ]  *)
+| red_sel1_l : forall x m s l y T ds,
+    binds x (val_new T ds) s ->
+    defs_has (open_defs x ds) (def_trm m (trm_var (avar_f y))) ->
+    (s, trm_sel (avar_f x) m, l) |->l (s, (trm_var (avar_f y)), l)
+
+| red_sel2_l : forall x m s t l T ds,
     binds x (val_new T ds) s ->
     defs_has (open_defs x ds) (def_trm m t) ->
-    (s, trm_sel (avar_f x) m) |-> (s, t)
+    (forall x, t <> (trm_var (avar_f x))) ->
+    (s, trm_sel (avar_f x) m, l) |->l (s, t, cons (x, m) l)
+
+| red_sel3_l : forall x m s s' s1 s2 l y T ds ds',
+    s = s1 & x ~ (val_new T ds) & s2 ->
+    s' = s1 & x ~ (val_new T ds') & s2 ->
+    (open_defs x ds') = (defs_update (open_defs x ds) m (trm_var (avar_f y))) ->
+    (s, (trm_var (avar_f y)), cons (x, m) l) |->l (s', (trm_var (avar_f y)), l)
 
 (** [s(x) = lambda(T)t]      #<br>#
     [―――――――――――――――――――――]  #<br>#
-    [(s, x y) |-> (s, t^y)]  *)
-| red_app : forall f a s T t,
+    [(s, x y) |->l (s, t^y)]  *)
+| red_app_l : forall f a s T t l,
     binds f (val_lambda T t) s ->
-    (s, trm_app (avar_f f) (avar_f a)) |-> (s, open_trm a t)
+    (s, trm_app (avar_f f) (avar_f a), l) |->l (s, open_trm a t, l)
 
-(** [(s, let x = v in t) |-> ((s, x = v), t^x)] *)
-| red_let_val : forall v t s x,
+(** [(s, let x = v in t) |->l ((s, x = v), t^x)] *)
+| red_let_val_l : forall v t s x l,
     x # s ->
-    (s, trm_let (trm_val v) t) |-> (s & x ~ v, open_trm x t)
+    (s, trm_let (trm_val v) t, l) |->l (s & x ~ v, open_trm x t, l)
 
-(** [(s, let y = x in t) |-> (s, t^x)] *)
-| red_let_var : forall t s x,
-    (s, trm_let (trm_var (avar_f x)) t) |-> (s, open_trm x t)
+(** [(s, let y = x in t) |->l (s, t^x)] *)
+| red_let_var_l : forall t s x l,
+    (s, trm_let (trm_var (avar_f x)) t, l) |->l (s, open_trm x t, l)
 
-(** [(s, t0) |-> (s', t0')]                             #<br>#
+(** [(s, t0) |->l (s', t0')]                             #<br>#
     [―――――――――――――――――――――――――――――――――――――――――――――――]  #<br>#
-    [(s, let x = t0 in t) |-> (s', let x = t0' in t)]  *)
-| red_let_tgt : forall t0 t s t0' s',
-    (s, t0) |-> (s', t0') ->
-    (s, trm_let t0 t) |-> (s', trm_let t0' t)
+    [(s, let x = t0 in t) |->l (s', let x = t0' in t)]  *)
+| red_let_tgt_l : forall t0 t s t0' s' l,
+    (s, t0, l) |->l (s', t0', l) ->
+    (s, trm_let t0 t, l) |->l (s', trm_let t0' t, l)
 
-where "t1 '|->' t2" := (red t1 t2).
+where "t1 '|->l' t2" := (red_l t1 t2).
 
-(** ** Normal forms *)
-(** Variables and values are considered to be in normal form. *)
-Inductive norm_form: trm -> Prop :=
-| nf_var: forall x, norm_form (trm_var x)
-| nf_val: forall v, norm_form (trm_val v).
-
-Hint Constructors red norm_form.
+Inductive norm_form_l: trm -> Prop :=
+| nf_var_l: forall x, norm_form_l (trm_var x).
