src/simple-proof/proof/Safety.v
@@ -3,15 +3,15 @@ Set Implicit Arguments.
 Require Import LibLN.
 Require Import Coq.Program.Equality.
 Require Import Binding CanonicalForms Definitions GeneralToTight InvertibleTyping Narrowing
-            OperationalSemantics PreciseTyping RecordAndInertTypes Substitution Weakening.
+        OperationalSemantics PreciseTyping RecordAndInertTypes Substitution Weakening.
 
 (** The typing of a term with a stack *)
-Inductive sta_trm_typ : sta * trm -> typ -> Prop :=
-| sta_trm_typ_c : forall G s t T,
+Inductive sta_trm_typ : sta * trm * call_stack -> typ -> Prop :=
+| sta_trm_typ_c : forall G s l t T,
     inert G ->
     well_typed G s ->
     G ⊢ t : T ->
-    sta_trm_typ (s, t) T.
+    sta_trm_typ (s, t, l) T.
 
 Hint Constructors sta_trm_typ.
 
@@ -42,17 +42,17 @@ Ltac binds_eq :=
 
 Ltac invert_red :=
   match goal with
-  | [Hr: (_, _) |-> (_, _) |- _] => inversions Hr
+  | [Hr: (_, _, _) |->l (_, _, _) |- _] => inversions Hr
   end.
 
 Ltac solve_IH :=
   match goal with
-  | [IH: well_typed _ _ ->
+  | [IH: well_typed_l _ _ ->
          inert _ ->
-         forall t', (_, _) |-> (_, _) -> _,
-       Wf: well_typed _ _,
+         forall t', (_, _) |->l (_, _) -> _,
+       Wf: well_typed_l _ _,
        In: inert _,
-       Hr: (_, _) |-> (_, ?t') |- _] =>
+       Hr: (_, _) |->l (_, ?t') |- _] =>
     specialize (IH Wf In t' Hr); destruct_all
   end;
   match goal with
@@ -65,7 +65,162 @@ Ltac solve_let :=
 
 (** [s: G]                  #<br>#
     [inert [G]              #<br>#
-    [(s, t) |-> (s', t')]   #<br>#
+    [(s, t) |->l (s', t')]   #<br>#
+    [G ⊢ t: T]              #<br>#
+    [―――――――――――――――――――]   #<br>#
+    [exists G', inert G']        #<br>#
+    [s': G, G']             #<br>#
+    [G, G' ⊢ t': T]         *)
+Lemma preservation_helper: forall G s t l s' t' l' T,
+    well_typed_l G s ->
+    inert G ->
+    (s, t, l) |->l (s', t', l') ->
+    G ⊢ t : T ->
+    exists G', inert G' /\
+          well_typed_l (G & G') s' /\
+          G & G' ⊢ t' : T.
+Proof.
+  introv Hwf Hin Hred Ht. gen t'.
+  induction Ht; intros; try solve [invert_red].
+  - Case "thunk_replace".
+    invert_red.
+    exists (@empty typ).
+    split; auto.
+    rewrite concat_empty_r; split; auto.
+    unfold well_typed_l in *.
+    destruct_all.
+    repeat split; try solve [simpl_dom; auto].
+    + eauto using ok_middle_change.
+    + intros.
+
+
+    intros.
+  - Case "ty_all_elim".
+    match goal with
+    | [Hx: _ ⊢ trm_var (avar_f _) : typ_all _ _ |- _] =>
+        pose proof (canonical_forms_fun Hin Hwf Hx) as [L [T' [t [Bis [Hsub Hty]]]]];
+          inversions Hred;
+          binds_eq
+    end.
+    exists (@empty typ). rewrite concat_empty_r. repeat split; auto.
+    pick_fresh y. assert (y \notin L) as FrL by auto. specialize (Hty y FrL).
+    eapply renaming_typ; eauto.
+  - Case "ty_new_elim".
+    pose proof (canonical_forms_obj Hin Hwf Ht) as [S [ds [t [Bis [Has Ty]]]]].
+    invert_red. binds_eq.
+    exists (@empty typ). rewrite concat_empty_r. repeat split; auto.
+    match goal with
+    | [Hd: defs_has _ (def_trm _ ?t') |- G ⊢ t': T] =>
+      rewrite* <- (defs_has_inv Has Hd)
+    end.
+  - Case "ty_let".
+    destruct t; try solve [solve_let].
+    + SCase "[t = (let x = a in u)] where a is a variable".
+      repeat invert_red.
+      exists (@empty typ). rewrite concat_empty_r. repeat split; auto.
+      apply* renaming_fresh.
+    + SCase "[t = (let x = v in u)] where v is a value".
+      repeat invert_red.
+      match goal with
+        | [Hn: ?x # ?s |- _] =>
+          pose proof (well_typed_notin_dom Hwf Hn) as Hng
+      end.
+      pose proof (val_typing Ht) as [V [Hv Hs]].
+      exists (x ~ V). repeat split.
+      ** rewrite <- concat_empty_l. constructor~. apply (precise_inert_typ Hv).
+      ** constructor~. apply (precise_to_general_v Hv).
+      ** eapply renaming_fresh with (L:=L \u dom G \u \{x}). apply* ok_push.
+         intros. apply* weaken_rules. apply ty_sub with (T:=V); auto. apply* weaken_subtyp.
+  - Case "ty_sub".
+    solve_IH.
+    match goal with
+    | [Hs: _ ⊢ _ <: _,
+       Hg: _ & ?G' ⊢ _: _ |- _] =>
+      apply weaken_subtyp with (G2:=G') in Hs;
+      eauto
+    end.
+Qed.
+
+(** ** Preservation Theorem *)
+
+(** [⊢ (s, t): T]           #<br>#
+    [(s, t) |->l (s', t')]   #<br>#
+    [―――――――――――――――――――]   #<br>#
+    [⊢ (s', t'): T]         *)
+Theorem preservation : forall s s' t t' T,
+    ⊢ (s, t) : T ->
+    (s, t) |->l (s', t') ->
+    ⊢ (s', t') : T.
+Proof.
+  introv Ht Hr. destruct Ht as [* Hi Hwf Ht].
+  lets Hp: (preservation_helper Hwf Hi Hr Ht). destruct Hp as [G' [Hi' [Hwf' Ht']]].
+  apply sta_trm_typ_c with (G:=G & G'); auto. apply* inert_concat.
+Qed.
+
+(** * Progress *)
+
+(** Helper tactic for proving progress *)
+Ltac solve_let_prog :=
+  match goal with
+      | [IH: ⊢ (?s, ?t) : ?T ->
+             inert _ ->
+             well_typed _ _ -> _,
+         Hi: inert _,
+         Hwt: well_typed _ _ |- _] =>
+        assert (⊢ (s, t): T) as Hs by eauto;
+        specialize (IH Hs Hi Hwt) as [IH | [s' [t' Hr]]];
+        eauto; inversion IH
+      end.
+
+(** ** Progress Theorem *)
+
+(** [⊢ (s, t): T]           #<br>#
+    [(s, t) |->l (s', t')]   #<br>#
+    [―――――――――――――――――――]   #<br>#
+    [t] is in normal form   #<br>#
+    or [exists s', t'] such that [(s, t) |->l (s', t')] *)
+Theorem progress: forall s t T,
+    ⊢ (s, t) : T ->
+    norm_form t \/ exists s' t', (s, t) |->l (s', t').
+Proof.
+  introv Ht. inversion Ht as [G s' t' T' Hi Hwt HT]. subst.
+  induction HT; eauto.
+  - Case "ty_all_elim".
+    pose proof (canonical_forms_fun Hi Hwt HT1). destruct_all. right*.
+  - Case "ty_new_elim".
+    pose proof (canonical_forms_obj Hi Hwt HT). destruct_all. right*.
+  - Case "ty_let".
+    right. destruct t; try solve [solve_let_prog].
+    + pose proof (var_typing_implies_avar_f HT) as [x A]. subst*.
+    + pick_fresh x. exists (s & x ~ v) (open_trm x u). auto.
+Qed.
+
+Ltac invert_red_l :=
+  match goal with
+  | [Hr: (_, _) |->ll (_, _) |- _] => inversions Hr
+  end.
+
+Ltac solve_IH :=
+  match goal with
+  | [IH: well_typed _ _ ->
+         inert _ ->
+         forall t', (_, _) |->ll (_, _) -> _,
+       Wf: well_typed _ _,
+       In: inert _,
+       Hr: (_, _) |->ll (_, ?t') |- _] =>
+    specialize (IH Wf In t' Hr); destruct_all
+  end;
+  match goal with
+  | [Hi: _ & ?G' ⊢ _ : _ |- _] =>
+    exists G'; repeat split; auto
+  end.
+
+Ltac solve_let :=
+  invert_red; solve_IH; fresh_constructor; eauto; apply* weaken_rules.
+
+(** [s: G]                  #<br>#
+    [inert [G]              #<br>#
+    [(s, t) |->l (s', t')]   #<br>#
     [G ⊢ t: T]              #<br>#
     [―――――――――――――――――――]   #<br>#
     [exists G', inert G']        #<br>#
@@ -74,7 +229,7 @@ Ltac solve_let :=
 Lemma preservation_helper: forall G s t s' t' T,
     well_typed G s ->
     inert G ->
-    (s, t) |-> (s', t') ->
+    (s, t) |->l (s', t') ->
     G ⊢ t : T ->
     exists G', inert G' /\
           well_typed (G & G') s' /\
@@ -131,12 +286,12 @@ Qed.
 (** ** Preservation Theorem *)
 
 (** [⊢ (s, t): T]           #<br>#
-    [(s, t) |-> (s', t')]   #<br>#
+    [(s, t) |->l (s', t')]   #<br>#
     [―――――――――――――――――――]   #<br>#
     [⊢ (s', t'): T]         *)
 Theorem preservation : forall s s' t t' T,
     ⊢ (s, t) : T ->
-    (s, t) |-> (s', t') ->
+    (s, t) |->l (s', t') ->
     ⊢ (s', t') : T.
 Proof.
   introv Ht Hr. destruct Ht as [* Hi Hwf Ht].
@@ -162,13 +317,13 @@ Ltac solve_let_prog :=
 (** ** Progress Theorem *)
 
 (** [⊢ (s, t): T]           #<br>#
-    [(s, t) |-> (s', t')]   #<br>#
+    [(s, t) |->l (s', t')]   #<br>#
     [―――――――――――――――――――]   #<br>#
     [t] is in normal form   #<br>#
-    or [exists s', t'] such that [(s, t) |-> (s', t')] *)
+    or [exists s', t'] such that [(s, t) |->l (s', t')] *)
 Theorem progress: forall s t T,
     ⊢ (s, t) : T ->
-    norm_form t \/ exists s' t', (s, t) |-> (s', t').
+    norm_form t \/ exists s' t', (s, t) |->l (s', t').
 Proof.
   introv Ht. inversion Ht as [G s' t' T' Hi Hwt HT]. subst.
   induction HT; eauto.
